platform/cito/examples/ExampleRepInv.v
@@ -1,21 +1,19 @@
 Set Implicit Arguments.
 
 Require Import AutoSep.
-Require Import WordMap.
 Require Import ExampleADT.
 Import ExampleADT.ExampleADT.
 Require Import RepInv.
 
 Parameter is_fset : W -> WordSet.t -> HProp.
-Parameter is_fmap : W -> WordMap.t W -> HProp.
 
-Require Import Cell SimpleCell.
+Require Import Cell SimpleCell Seq ArraySeq.
 
 Definition rep_inv p adtvalue : HProp :=
   match adtvalue with
-    | FSet s => is_fset p s
-    | FMap m => is_fmap p m
     | Cell v => cell v p
+    | Arr ws => arr ws p
+    | FSet s => is_fset p s
   end.
 
 Module ExampleRepInv <: RepInv ExampleADT.
@@ -26,9 +24,9 @@ Module ExampleRepInv <: RepInv ExampleADT.
 
   Lemma rep_inv_ptr : forall p a, rep_inv p a ===> p =?> 1 * any.
     destruct a; simpl.
-    admit.
-    admit.
     eapply Himp_trans; [ apply cell_fwd | sepLemma ]; apply any_easy.
+    eapply Himp_trans; [ apply arr_fwd | sepLemma ]; apply any_easy.
+    admit.
   Qed.
 
 End ExampleRepInv.
